---
layout:     post
catalog: true
title:      A short proof for Nesterov’s momentum
subtitle:      转载自：https://blogs.princeton.edu/imabandit/2018/11/21/a-short-proof-for-nesterovs-momentum/
date:      2018-11-21
author:      Sebastien Bubeck
tags:
    - visible tweet
    - posted
    - inequalities
    - inequality
    - momentum
---

Yesterday I posted the following picture on Twitter and it quickly became my most visible tweet ever (by far):

     ![](https://i1.wp.com/blogs.princeton.edu/imabandit/wp-content/ql-cache/quicklatex.com-d2bae84ef1d0f3d68395b2753051452d_l3.png?resize=589%2C155&ssl=1)


I thought this would be a good opportunity to revisit the proof of Nesterov’s momentum, especially since as it turns out I really don’t like the way I described it back in 2013 (and to this day the latter post also remains my most visible post ever…). So here we go, for what is hopefully a short and intuitive proof of the ![](https://i0.wp.com/blogs.princeton.edu/imabandit/wp-content/ql-cache/quicklatex.com-cd0c1962105a4d25ae10283b6102d5e7_l3.png?resize=30%2C20&ssl=1)
 convergence rate for Nesterov’s momentum (disclaimer: this proof is merely a rearranging of well-known calculations, nothing new is going on here).

We assume that ![](https://i1.wp.com/blogs.princeton.edu/imabandit/wp-content/ql-cache/quicklatex.com-c7d97b919a3b73617cf2fbb375fff3b1_l3.png?resize=10%2C16&ssl=1)
 is ![](https://i2.wp.com/blogs.princeton.edu/imabandit/wp-content/ql-cache/quicklatex.com-874e8d85c668e484f7277da3d75ce10e_l3.png?resize=11%2C16&ssl=1)
-smooth convex function, and we take ![](https://i2.wp.com/blogs.princeton.edu/imabandit/wp-content/ql-cache/quicklatex.com-c22ff34deb301bf7b54eaa30c554a872_l3.png?resize=62%2C18&ssl=1)
 in the gradient step. The momentum term ![](https://i2.wp.com/blogs.princeton.edu/imabandit/wp-content/ql-cache/quicklatex.com-489a425d5327168dba48971817ba248e_l3.png?resize=14%2C12&ssl=1)
 will be set to a very particular value, which comes out naturally in the proof.

 

**The two basic inequalities**

Let us denote ![](https://i1.wp.com/blogs.princeton.edu/imabandit/wp-content/ql-cache/quicklatex.com-f3e2fbe422fdee3fa63839629f24f09a_l3.png?resize=155%2C25&ssl=1)
 (note that ![](https://i1.wp.com/blogs.princeton.edu/imabandit/wp-content/ql-cache/quicklatex.com-14f53a34ec75692ebeb7979c4b789e0b_l3.png?resize=145%2C18&ssl=1)
). Now let us write our favorite inequalities (using ![](https://i2.wp.com/blogs.princeton.edu/imabandit/wp-content/ql-cache/quicklatex.com-6c0cf4bdbacb7b59c2f14a4c6c939d71_l3.png?resize=225%2C25&ssl=1)
 and ![](https://i1.wp.com/blogs.princeton.edu/imabandit/wp-content/ql-cache/quicklatex.com-1e5ece4005951fee2314a4aa9fc0b472_l3.png?resize=230%2C18&ssl=1)
):

     ![](https://i1.wp.com/blogs.princeton.edu/imabandit/wp-content/ql-cache/quicklatex.com-2f2a79eecb14e19584aa14a21015245c_l3.png?resize=253%2C36&ssl=1)


and

     ![](https://i1.wp.com/blogs.princeton.edu/imabandit/wp-content/ql-cache/quicklatex.com-dfb5d94574f3f51e375702a6aa2273a3_l3.png?resize=308%2C36&ssl=1)


 

**On the way to a telescopic sum**

Recall now that ![](https://i2.wp.com/blogs.princeton.edu/imabandit/wp-content/ql-cache/quicklatex.com-f9a7eb15608470b13b9314248a7ff3aa_l3.png?resize=212%2C19&ssl=1)
, so it would be nice to somehow combine the two above inequalities to obtain a telescopic sum thanks to this simple formula. Let us try to take a convex combination of the two inequalities. In fact it will be slightly more elegant if we use the coefficient ![](https://i0.wp.com/blogs.princeton.edu/imabandit/wp-content/ql-cache/quicklatex.com-21b5b4cbe9a10b6d847eeb4265b99898_l3.png?resize=7%2C13&ssl=1)
 on the second inequality, so let us do ![](https://i2.wp.com/blogs.princeton.edu/imabandit/wp-content/ql-cache/quicklatex.com-1a681cd9587084897fd82bc5a2b7e5c9_l3.png?resize=46%2C15&ssl=1)
 times the first inequality plus ![](https://i0.wp.com/blogs.princeton.edu/imabandit/wp-content/ql-cache/quicklatex.com-21b5b4cbe9a10b6d847eeb4265b99898_l3.png?resize=7%2C13&ssl=1)
 times the second inequality. We obtain an inequality whose right hand side is given by ![](https://i1.wp.com/blogs.princeton.edu/imabandit/wp-content/ql-cache/quicklatex.com-3c4a581d257fd68c4d9c37a1c333db77_l3.png?resize=24%2C23&ssl=1)
 times

     ![](https://i0.wp.com/blogs.princeton.edu/imabandit/wp-content/ql-cache/quicklatex.com-add8691a09d680d0a59cb09eec7035d7_l3.png?resize=398%2C68&ssl=1)


Recall that our objective is to obtain a telescopic sum, and at this point we still have flexibility both to choose ![](https://i1.wp.com/blogs.princeton.edu/imabandit/wp-content/ql-cache/quicklatex.com-9c908ff5ec1398a4aa9a734884c60e9f_l3.png?resize=15%2C15&ssl=1)
 and ![](https://i2.wp.com/blogs.princeton.edu/imabandit/wp-content/ql-cache/quicklatex.com-489a425d5327168dba48971817ba248e_l3.png?resize=14%2C12&ssl=1)
. What we would like to have is:

     ![](https://i1.wp.com/blogs.princeton.edu/imabandit/wp-content/ql-cache/quicklatex.com-77cfa389a4eb920bef5425d09daa5b58_l3.png?resize=351%2C19&ssl=1)


Observe that (since ![](https://i2.wp.com/blogs.princeton.edu/imabandit/wp-content/ql-cache/quicklatex.com-232e22af86eadf45ef59fa880dea2b4a_l3.png?resize=151%2C26&ssl=1)
) the right hand side can be written as ![](https://i1.wp.com/blogs.princeton.edu/imabandit/wp-content/ql-cache/quicklatex.com-0f0d7099917cc6d61bb00c0c373c7167_l3.png?resize=245%2C28&ssl=1)
, and thus we see that we simply need to have:

     ![](https://i0.wp.com/blogs.princeton.edu/imabandit/wp-content/ql-cache/quicklatex.com-6d02c948f048b8068b001318943afcc7_l3.png?resize=115%2C40&ssl=1)


 

**Setting the parameters and concluding the proof**

Writing ![](https://i2.wp.com/blogs.princeton.edu/imabandit/wp-content/ql-cache/quicklatex.com-a738d10d455ab56707e24cda611ff4d0_l3.png?resize=182%2C23&ssl=1)
 we now obtain as a result of the combination of our two starting inequalities:

     ![](https://i0.wp.com/blogs.princeton.edu/imabandit/wp-content/ql-cache/quicklatex.com-07e4430c91aa1bd339a32f5c5fbfa3cc_l3.png?resize=256%2C21&ssl=1)


It only remains to select ![](https://i1.wp.com/blogs.princeton.edu/imabandit/wp-content/ql-cache/quicklatex.com-9c908ff5ec1398a4aa9a734884c60e9f_l3.png?resize=15%2C15&ssl=1)
 such that ![](https://i2.wp.com/blogs.princeton.edu/imabandit/wp-content/ql-cache/quicklatex.com-8287b288ecb0f9cbd00fbd4c6f903455_l3.png?resize=111%2C19&ssl=1)
 (i.e., roughly ![](https://i1.wp.com/blogs.princeton.edu/imabandit/wp-content/ql-cache/quicklatex.com-9c908ff5ec1398a4aa9a734884c60e9f_l3.png?resize=15%2C15&ssl=1)
 is of order ![](https://i2.wp.com/blogs.princeton.edu/imabandit/wp-content/ql-cache/quicklatex.com-6b97bb0f65c75b6cc0fba1868749478d_l3.png?resize=6%2C12&ssl=1)
) so that by summing the previous inequality one obtains ![](https://i0.wp.com/blogs.princeton.edu/imabandit/wp-content/ql-cache/quicklatex.com-0ad08a0fcdfd8cb6ec6f7f579b5dc417_l3.png?resize=120%2C30&ssl=1)
 which is exactly the ![](https://i0.wp.com/blogs.princeton.edu/imabandit/wp-content/ql-cache/quicklatex.com-cd0c1962105a4d25ae10283b6102d5e7_l3.png?resize=30%2C20&ssl=1)
 rate we were looking for.
